add more renaming bits

LeanSubst/Class.lean
@@ -32,41 +32,83 @@ instance (priority := high) [RenMap T T] [RenMapCompose T T] : RenMapCompose (Ac
 instance [RenMap S T] [RenMapCompose S T] : RenMapCompose (Action S) T where
   apply_compose := by intro s; cases s <;> simp
 
-class SubstMapId (S : Type u1) (T : Type u2) [SubstMap S T] where
-  apply_id {s : S} : s[.id T] = s
-
 class SubstMapStable (S : Type u1) (T : Type u2) [RenMap S T] [SubstMap S T] where
   apply_stable (r : Ren T) (σ : Subst T) : r.to = σ -> rmap (S := S) r = smap σ
+
+class SubstMapId (S : Type u1) (T : Type u2) [SubstMap S T] where
+  apply_id {s : S} : s[.id T] = s
 
 class SubstMapRenComposeLeft (S : Type u1) (T : Type u2) [RenMap S T] [SubstMap S T] where
   apply_ren_compose_left {s : S} {r : Ren T} {τ : Subst T} : s⟨r⟩[τ] = s[r ∘ τ]
 
-class SubstMapRenComposeRight (T : Type u2) [RenMap T T] [SubstMap T T] where
-  apply_ren_compose_right {t : T} {r : Ren T} {σ : Subst T} : t[σ]⟨r⟩ = t[σ ∘ r]
+class SubstMapRenComposeRight (S : Type u1) (T : Type u2) [RenMap S T] [RenMap T T] [SubstMap S T] where
+  apply_ren_compose_right {s : S} {r : Ren T} {σ : Subst T} : s[σ]⟨r⟩ = s[σ ∘ r]
 
 class SubstMapCompose (S : Type u1) (T : Type u2) [SubstMap S T] [SubstMap T T] where
   apply_compose {s : S} {σ τ : Subst T} : s[σ][τ] = s[σ ∘ τ]
 
-class SubstMapRenCommute (S : Type u1) (T : Type u2) [RenMap S S] [SubstMap S T] where
-  apply_ren_commute {s : S} (r : Ren S) (τ : Subst T) : s⟨r⟩[τ] = s[τ]⟨r⟩
+class SubstMapRenCommute (S : Type u1) (T : Type u2) [RenMap S S] [RenMap S T] [SubstMap S T] where
+  apply_commute_ren_subst {s : S} {r : Ren S} {τ : Subst T} : s⟨r⟩[τ] = s[τ]⟨r⟩
+  apply_commute_ren_ren {s : S} {r1 : Ren S} {r2 : Ren T} : s⟨r1⟩⟨r2⟩ = s⟨r2⟩⟨r1⟩
+
+class SubstMapRenHetCompose (S : Type u1) (T : Type u2) [RenMap S T] [SubstMap S S] where
+  apply_hcompose_ren {s : S} {σ : Subst S} {r : Ren T} : s[σ]⟨r⟩ = s⟨r⟩[σ ◾ r]
 
 class SubstMapHetCompose (S : Type u1) (T : Type u2) [SubstMap S S] [SubstMap S T] where
   apply_hcompose {s : S} {σ : Subst S} {τ : Subst T} : s[σ][τ] = s[τ][σ ◾ τ]
 
-namespace Subst
-  export SubstMapStable (apply_stable)
-  export SubstMapRenComposeLeft (apply_ren_compose_left)
-  export SubstMapRenComposeRight (apply_ren_compose_right)
-  export SubstMapRenCommute (apply_ren_commute)
-end Subst
+theorem Subst.apply_stable
+  [RenMap S T] [SubstMap S T] [SubstMapStable S T]
+  {r : Ren T} {σ : Subst T}
+  : r.to = σ -> rmap (S := S) r = smap σ
+:= SubstMapStable.apply_stable _ _
 
 @[simp, grind =]
 theorem Subst.apply_id [SubstMap S T] [SubstMapId S T] {s : S} : s[.id T] = s := SubstMapId.apply_id
+
+@[simp, grind =]
+theorem Subst.apply_ren_compose_left [RenMap S T] [SubstMap S T] [SubstMapRenComposeLeft S T]
+  {s : S} {r : Ren T} {τ : Subst T}
+  : s⟨r⟩[τ] = s[r ∘ τ]
+:= SubstMapRenComposeLeft.apply_ren_compose_left
+
+@[simp, grind =]
+theorem Subst.apply_ren_compose_right
+  [RenMap S T] [RenMap T T] [SubstMap S T] [SubstMapRenComposeRight S T]
+  {s : S} {σ : Subst T} {r : Ren T}
+  : s[σ]⟨r⟩ = s[σ ∘ r]
+:= SubstMapRenComposeRight.apply_ren_compose_right
+
+@[grind =]
+theorem Subst.apply_commute_ren_subst
+  [RenMap S S] [RenMap S T] [SubstMap S T] [SubstMapRenCommute S T]
+  {s : S} {r : Ren S} {τ : Subst T}
+  : s⟨r⟩[τ] = s[τ]⟨r⟩
+:= SubstMapRenCommute.apply_commute_ren_subst
+
+@[grind =]
+theorem Subst.apply_commute_ren_ren
+  [RenMap S S] [RenMap S T] [SubstMap S T] [SubstMapRenCommute S T]
+  {s : S} {r1 : Ren S} {r2 : Ren T}
+  : s⟨r1⟩⟨r2⟩ = s⟨r2⟩⟨r1⟩
+:= SubstMapRenCommute.apply_commute_ren_ren
 
 @[simp, grind =]
 theorem Subst.apply_compose [SubstMap S T] [SubstMap T T] [SubstMapCompose S T]
   {s : S} {σ τ : Subst T}
   : s[σ][τ] = s[σ ∘ τ]
 := SubstMapCompose.apply_compose
+
+@[simp, grind =]
+theorem Subst.apply_hcompose_ren [SubstMap S S] [RenMap S T] [SubstMapRenHetCompose S T]
+  {s : S} {σ : Subst S} {r : Ren T}
+  : s[σ]⟨r⟩ = s⟨r⟩[σ ◾ r]
+:= SubstMapRenHetCompose.apply_hcompose_ren
+
+@[simp, grind =]
+theorem Subst.apply_hcompose [SubstMap S S] [SubstMap S T] [SubstMapHetCompose S T]
+  {s : S} {σ : Subst S} {τ : Subst T}
+  : s[σ][τ] = s[τ][σ ◾ τ]
+:= SubstMapHetCompose.apply_hcompose
 
 end LeanSubst
