LeanSubst/Laws.lean
@@ -17,24 +17,39 @@ theorem Ren.lift_eq_from_eq [RenMap T T] {r : Ren T} {σ : Subst T}
 
 namespace Subst
   section
+    @[simp]
+    theorem rewrite0 [RenMap T T] : +0σ ∘ +1r = succ T := by
+      congr
+
     @[simp, grind =]
-    theorem rewrite1 : re 0 :: +1 = id T := by
+    theorem rewrite1 : re 0 :: +1σ = id T := by
       simp [Subst.cons, Subst.id]
       funext; case _ x =>
       cases x; all_goals simp
 
+    @[simp, grind =]
+    theorem rewrite1_ren : 0 :: +1r = Ren.id T := by
+      simp [Ren.cons, Ren.id]
+      funext; case _ x =>
+      cases x <;> simp
+
     open SubstMap
 
     @[simp, grind =]
-    theorem I_lift [RenMap T T] {k} : +0.lift k = id T := by
+    theorem I_lift [RenMap T T] {k} : +0σ.lift k = id T := by
       funext; case _ x =>
       cases x; all_goals (simp [lift, id, act, SubstAction.act])
       grind
 
     @[simp, grind =]
-    theorem rewrite2 [SubstMap T T] {σ : Subst T} : +0 ∘ σ = σ := by
+    theorem rewrite2 [SubstMap T T] {σ : Subst T} : +0σ ∘ σ = σ := by
       funext; case _ x =>
       simp [compose, id, act, SubstAction.act]
+
+    @[simp, grind =]
+    theorem rewrite2_ren [SubstMap T T] {σ : Subst T} : +0r ∘ σ = σ := by
+      funext; case _ x =>
+      simp [compose_ren_left, act, SubstAction.act]
 
     @[simp, grind =]
     theorem rewrite3_cons [SubstMap T T] {σ τ : Subst T} {a : Action T}
@@ -74,33 +89,37 @@ namespace Subst
       cases hd <;> simp [*]
 
     @[simp, grind =]
-    theorem rewrite4_cons [SubstMap T T]  {s} {σ : Subst T} : +1 ∘ (s :: σ) = σ := by
+    theorem rewrite4_cons [SubstMap T T]  {s} {σ : Subst T} : +1σ ∘ (s :: σ) = σ := by
       simp [Subst.cons]
       funext; case _ x =>
       cases x; all_goals (simp [compose, succ, act, SubstAction.act])
 
     @[simp, grind =]
-    theorem rewrite5 [SubstMap T T] {σ : Subst T} : σ.act 0 :: (+1 ∘ σ) = σ := by
+    theorem rewrite4_cons_ren [SubstMap T T]  {s} {σ : Subst T} : +1r ∘ (s :: σ) = σ := by
+      simp [Subst.cons]
+      funext; case _ x =>
+      cases x; all_goals (simp [compose_ren_left, act, SubstAction.act])
+
+    @[simp, grind =]
+    theorem rewrite5 [SubstMap T T] {σ : Subst T} : σ.act 0 :: (+1σ ∘ σ) = σ := by
       simp [Subst.cons, Subst.compose]; congr
+      funext; case _ x =>
+      cases x <;> simp [act, SubstAction.act]
+
+    @[simp, grind =]
+    theorem rewrite5_ren [SubstMap T T] {σ : Subst T} : σ.act 0 :: (+1r ∘ σ) = σ := by
+      simp [Subst.cons]; congr
       funext; case _ x =>
       cases x <;> simp [act, SubstAction.act]
   end
 
   @[simp, grind =]
-  theorem rewrite_lift [RenMap T T] [SubstMap T T] [SubstMapStable T T] {σ : Subst T}
-    : σ.lift = re 0 :: (σ ∘ +1)
+  theorem rewrite_lift [RenMap T T] {σ : Subst T}
+    : σ.lift = re 0 :: (σ ∘ +1r)
   := by
-    simp [Subst.cons, Subst.lift, Subst.compose]
+    simp [cons, lift, compose_ren_right]
     funext; case _ x =>
-    cases x; simp
-    case _ n =>
-      simp [Subst.succ, act, SubstAction.act]
-      generalize tdef : σ.inner n = t
-      cases t <;> simp [act, SubstAction.act] at *
-      case _ y =>
-        rw [apply_stable (σ := +1)]
-        simp [Subst.succ]
-        rw [Ren.to_succ]
+    cases x <;> simp
 
   @[simp, grind =]
   theorem rewrite_lift_zero [RenMap T T] [RenMapId T T] {σ : Subst T}
@@ -126,7 +145,7 @@ namespace Subst
 
   @[simp, grind =]
   theorem rewrite6 [RenMap T T] [SubstMap T T] [SubstMapId T T] {σ : Subst T}
-    : σ ∘ +0 = σ
+    : σ ∘ +0σ = σ
   := by
     simp [compose, id, act, SubstAction.act]; congr; funext; case _ x =>
     generalize zdef : σ.inner x = z
@@ -134,6 +153,12 @@ namespace Subst
     case _ t =>
     have lem : t[id T] = t := by simp
     simp [id] at lem; exact lem
+
+  @[simp, grind =]
+  theorem rewrite6_ren [RenMap T T] [RenMapId T T] {σ : Subst T}
+    : σ ∘ +0r = σ
+  := by
+    simp [compose_ren_right]; congr
 
   @[simp, grind =]
   theorem rewrite7
@@ -145,6 +170,13 @@ namespace Subst
     funext; case _ x =>
     cases σ.inner x <;> simp [act, SubstAction.act]
     simp [compose, act, SubstAction.act]
+
+  @[simp, grind =]
+  theorem rewrite7_ren
+    [RenMap T T] [RenMapCompose T T]
+    {σ : Subst T} {r1 r2 : Ren T}
+    : (σ ∘ r1) ∘ r2 = σ ∘ r1 ∘ r2
+  := by simp [compose_ren_right]
 
   @[simp, grind =]
   theorem rewrite4_append_direct [SubstMap T T] [SubstMapCompose T T]
@@ -161,34 +193,6 @@ namespace Subst
     {k} {ℓ : List $ Action T} {σ : Subst T} (h : k = ℓ.length)
     : (add T k) ∘ (ℓ ++ σ) = σ
   := by subst h; simp
-
-  -- @[simp]
-  -- theorem list_act_id {ℓ : List Nat} {σ : Subst T} : act (id T) ℓ ++ σ = ℓ ++ σ := sorry
-
-  -- @[simp]
-  -- theorem list_append_range_0 {σ : Subst T}
-  --   : List.range 0 ++ σ = σ
-  -- := by simp
-
-  -- @[simp]
-  -- theorem list_append_range_add {σ : Subst T} {n k}
-  --   : List.range (n + k) ++ σ = List.range k ++ (((add T k).act $ List.range n) ++ σ)
-  -- := by
-  --   induction k generalizing n σ; simp
-  --   case _ k ih =>
-
-  --     sorry
-
-  -- @[simp]
-  -- theorem list_append_range_succ {σ : Subst T} {n}
-  --   : List.range (n + 1) ++ σ = re 0 :: ((succ T).act $ List.range n) ++ σ
-  -- := by
-  --   generalize zdef : List.range (n + 1) = z at *
-  --   induction z generalizing n σ <;> simp
-  --   case _ =>
-  --     sorry
-  --   case _ hd tl ih =>
-  --     sorry
 
   @[grind =]
   theorem subst_append_assoc {xs ys : List $ Action T} {σ : Subst T}
@@ -223,18 +227,40 @@ namespace Subst
         case _ h4 => rw [subst_append_assoc_nat]; simp
         case _ h4 => omega
 
+  @[simp]
+  theorem range_act_succ_ren {s e : Nat} {σ : Subst T}
+    : (s..e)⟨.succ T⟩ ++ σ = s.succ..e.succ ++ σ
+  := by
+    induction e generalizing s σ <;> simp
+    case _ e ih =>
+    simp [Ren.range]
+    cases Nat.decLe s e
+    case _ h2 => simp [ite]
+    case _ h2 =>
+      simp [ite]
+      cases Nat.decLe (s + 1) e
+      case _ h3 =>
+        have lem : s = e := by omega
+        subst lem; simp
+      case _ h3 =>
+        simp [*]
+        rw [subst_append_assoc_nat, ih]; simp
+        rw [subst_append_assoc_nat]; simp [Ren.range]
+        split
+        case _ h4 => rw [subst_append_assoc_nat]; simp
+        case _ h4 => omega
+
   @[simp, grind =]
   theorem rewrite_lift_k
-    [RenMap T T] [RenMapId T T] [RenMapCompose T T] [SubstMap T T] [SubstMapId T T]
-    [SubstMapStable T T] [SubstMapCompose T T]
+    [RenMap T T] [RenMapId T T] [RenMapCompose T T]
+    [SubstMap T T] [SubstMapId T T] [SubstMapCompose T T]
     {k} {σ : Subst T}
-    : σ.lift k = 0..k ++ (σ ∘ add T k)
+    : σ.lift k = 0..k ++ (σ ∘ +r k)
   := by
-    induction k generalizing σ; simp
+    induction k generalizing σ <;> simp
     case _ k ih =>
       rw [rewrite_lift_succ, ih]
-      rw [compose_add_succ_right]
-      simp
+      simp; congr
 
   @[simp, grind =]
   theorem hrewrite1 [SubstMap S T] [SubstMapId S T] {σ : Subst S} : σ ◾ (id T) = σ := by
@@ -243,22 +269,25 @@ namespace Subst
     generalize zdef : σ.inner x = z
     cases z <;> simp
 
-  -- @[simp, grind =]
-  -- theorem hcomp_ren_left
-  --   [RenMap S] [RenMap T] [SubstMap S T]
-  --   (r : Ren) (σ : Subst T)
-  --   : (@Ren.to S r) ◾ σ = r.to
-  -- := by
-  --   funext; case _ x =>
-  --   induction x <;> simp [Subst.hcompose, Ren.to]
+  @[simp, grind =]
+  theorem hrewrite1_ren [RenMap S T] [RenMapId S T] {σ : Subst S} : σ ◾ (.id T) = σ := by
+    simp [hcompose_ren, act, SubstAction.act]
 
   @[simp, grind =]
-  theorem hrewrite2 [SubstMap S T] {σ : Subst T} : (id S) ◾ σ = +0 := by
+  theorem hrewrite2 [SubstMap S T] {σ : Subst T} : (id S) ◾ σ = +0σ := by
     simp [hcompose, id, act, SubstAction.act]
 
   @[simp, grind =]
-  theorem hrewrite3 [SubstMap S T] {σ : Subst T} : (succ S) ◾ σ = +1 := by
+  theorem hrewrite2_ren [RenMap S T] {r : Ren T} : (id S) ◾ r = +0σ := by
+    simp [hcompose_ren, id, act, SubstAction.act]
+
+  @[simp, grind =]
+  theorem hrewrite3 [SubstMap S T] {σ : Subst T} : (succ S) ◾ σ = +1σ := by
     simp [hcompose, succ, act, SubstAction.act]
+
+  @[simp, grind =]
+  theorem hrewrite3_ren [RenMap S T] {r : Ren T} : (succ S) ◾ r = +1σ := by
+    simp [hcompose_ren, succ, act, SubstAction.act]
 
   @[simp, grind =]
   theorem hrewrite4
@@ -267,6 +296,16 @@ namespace Subst
     : (re x :: σ) ◾ τ = re x :: (σ ◾ τ)
   := by
     simp [Subst.hcompose, act]; congr
+    funext; case _ i =>
+    cases i <;> simp [Subst.cons, act, SubstAction.act]
+
+  @[simp, grind =]
+  theorem hrewrite4_ren
+    [RenMap S T]
+    {x} {σ : Subst S} {r : Ren T}
+    : (re x :: σ) ◾ r = re x :: (σ ◾ r)
+  := by
+    simp [hcompose_ren, act]; congr
     funext; case _ i =>
     cases i <;> simp [Subst.cons, act, SubstAction.act]
 
@@ -280,7 +319,7 @@ namespace Subst
     simp [hcompose, compose_ren_left, act, SubstAction.act]
 
   @[simp, grind =]
-  theorem hrewrite5
+  theorem hrewrite5_subst_subst
     [SubstMap S T] [SubstMap T T] [SubstMapCompose S T]
     {σ : Subst S} {τ μ : Subst T}
     : (σ ◾ τ) ◾ μ = σ ◾ (τ ∘ μ)
@@ -290,23 +329,46 @@ namespace Subst
     generalize zdef : σ.inner x = z
     cases z <;> simp
 
+  @[simp, grind =]
+  theorem hrewrite5_subst_ren
+    [RenMap S T] [RenMap T T] [SubstMap S T] [SubstMapRenComposeRight S T]
+    {σ : Subst S} {τ : Subst T} {r : Ren T}
+    : (σ ◾ τ) ◾ r = σ ◾ (τ ∘ r)
+  := by
+    simp [hcompose_ren, hcompose, act, SubstAction.act]
+    funext; case _ x =>
+    generalize zdef : σ.inner x = z
+    cases z <;> simp
+
+  @[simp, grind =]
+  theorem hrewrite5_ren_subst
+    [RenMap S T] [SubstMap S T] [SubstMapRenComposeLeft S T]
+    {σ : Subst S} {τ : Subst T} {r : Ren T}
+    : (σ ◾ r) ◾ τ = σ ◾ (r ∘ τ)
+  := by
+    simp [hcompose_ren, hcompose, act, SubstAction.act]
+    funext; case _ x =>
+    generalize zdef : σ.inner x = z
+    cases z <;> simp
+
+  @[simp, grind =]
+  theorem hrewrite5_ren_ren
+    [RenMap S T] [SubstMap S T] [RenMapCompose S T]
+    {σ : Subst S} {r1 r2 : Ren T}
+    : (σ ◾ r1) ◾ r2 = σ ◾ (r1 ∘ r2)
+  := by
+    simp [hcompose_ren, act, SubstAction.act]
+
   @[grind =]
   theorem hcomp_distr_ren_right
-    [RenMap S S] [SubstMap S S] [SubstMap S T] [SubstMapRenCommute S T]
+    [RenMap S S] [RenMap S T] [SubstMap S S] [SubstMap S T] [SubstMapRenCommute S T]
     (r : Ren S) (σ : Subst S) (μ : Subst T)
     : (σ ∘ r) ◾ μ = (σ ◾ μ) ∘ r
   := by
     simp [hcompose, compose_ren_right, act, SubstAction.act]; funext; case _ x =>
     generalize zdef : σ.inner x = z
     cases z <;> simp
-    rw [apply_ren_commute]
-
-  @[simp, grind =]
-  theorem apply_hcompose
-    [SubstMap S S] [SubstMap S T] [SubstMapHetCompose S T]
-    {s : S} {σ : Subst S} {τ : Subst T}
-    : s[σ][τ] = s[τ][σ ◾ τ]
-  := by exact SubstMapHetCompose.apply_hcompose
+    rw [apply_commute_ren_subst]
 
   @[simp, grind =]
   theorem hrewrite7
@@ -314,13 +376,64 @@ namespace Subst
     {σ τ : Subst S} (μ : Subst T)
     : (σ ∘ τ) ◾ μ = (σ ◾ μ) ∘ τ ◾ μ
   := by
-    simp [Subst.hcompose, Subst.compose, act, SubstAction.act]
+    simp [hcompose, compose, act, SubstAction.act]
     funext; case _ x =>
     generalize zdef : σ.inner x = z
-    cases z <;> simp [Subst.hcompose, act, SubstAction.act]
+    cases z <;> simp [hcompose, act, SubstAction.act]
+
+  @[simp, grind =]
+  theorem hrewrite7_ren
+    [RenMap S S] [RenMap S T] [SubstMap S S] [SubstMap S T] [SubstMapRenHetCompose S T]
+    {σ τ : Subst S} {r : Ren T}
+    : (σ ∘ τ) ◾ r = (σ ◾ r) ∘ τ ◾ r
+  := by
+    simp [hcompose_ren, compose, act, SubstAction.act]
+    funext; case _ x =>
+    generalize zdef : σ.inner x = z
+    cases z <;> simp [hcompose_ren, act, SubstAction.act]
+
+  @[simp, grind =]
+  theorem hrewrite8
+    [SubstMap S S] [SubstMap S T]
+    {r : Ren S} {τ : Subst S} (μ : Subst T)
+    : (r ∘ τ) ◾ μ = r ∘ τ ◾ μ
+  := by
+    simp [hcompose, compose_ren_left, act, SubstAction.act]
+
+  @[simp, grind =]
+  theorem hrewrite8_ren
+    [RenMap S T] [SubstMap S S] [SubstMap S T]
+    {r : Ren S} {τ : Subst S} (μ : Ren T)
+    : (r ∘ τ) ◾ μ = r ∘ τ ◾ μ
+  := by
+    simp [hcompose_ren, compose_ren_left, act, SubstAction.act]
+
+  @[simp, grind =]
+  theorem hrewrite9
+    [RenMap S S] [RenMap S T] [SubstMap S S] [SubstMap S T] [SubstMapRenCommute S T]
+    {σ : Subst S} {r : Ren S} (μ : Subst T)
+    : (σ ∘ r) ◾ μ = (σ ◾ μ) ∘ r
+  := by
+    simp [hcompose, compose_ren_right, act, SubstAction.act]
+    funext; case _ x =>
+    generalize zdef : σ.inner x = z
+    cases z <;> simp
+    rw [apply_commute_ren_subst]
+
+  @[simp, grind =]
+  theorem hrewrite9_ren
+    [RenMap S S] [RenMap S T] [SubstMap S S] [SubstMap S T] [SubstMapRenCommute S T]
+    {σ : Subst S} {r : Ren S} (μ : Ren T)
+    : (σ ∘ r) ◾ μ = (σ ◾ μ) ∘ r
+  := by
+    simp [hcompose_ren, compose_ren_right, act, SubstAction.act]
+    funext; case _ x =>
+    generalize zdef : σ.inner x = z
+    cases z <;> simp
+    rw [apply_commute_ren_ren]
 
   theorem hrewrite_lift1
-    [RenMap S S] [SubstMap S S] [SubstMap S T] [SubstMapHetCompose S T] [SubstMapRenCommute S T]
+    [RenMap S S] [RenMap S T] [SubstMap S S] [SubstMap S T] [SubstMapRenCommute S T]
     {σ : Subst S} {τ : Subst T}
     : (σ ◾ τ).lift = σ.lift ◾ τ
   := by
@@ -330,12 +443,12 @@ namespace Subst
       simp [hcompose, act, SubstAction.act]
       generalize zdef : σ.inner n = z
       cases z <;> simp; case _ t =>
-      rw [SubstMapRenCommute.apply_ren_commute]
+      rw [apply_commute_ren_subst]
 
   @[simp, grind =]
   theorem hrewrite_lift
-    [RenMap S S] [SubstMap S S] [SubstMap S T] [RenMapId S S] [RenMapCompose S S]
-    [SubstMapHetCompose S T] [SubstMapRenCommute S T]
+    [RenMap S S] [RenMap S T] [SubstMap S S] [SubstMap S T]
+    [RenMapId S S] [RenMapCompose S S] [SubstMapRenCommute S T]
     {k} {σ : Subst S} {τ : Subst T}
     : (σ ◾ τ).lift k = σ.lift k ◾ τ
   := by
@@ -344,8 +457,35 @@ namespace Subst
     case _ i ih =>
       rw [rewrite_lift_succ]
       rw [rewrite_lift_succ]
-      simp; rw [ih, hrewrite_lift1]
+      simp; rw [ih]
       grind
+
+  theorem hrewrite_lift1_ren
+    [RenMap S S] [SubstMap S S] [RenMap S T] [SubstMap S T] [SubstMapRenCommute S T]
+    {σ : Subst S} {τ : Ren T}
+    : (σ ◾ τ).lift = σ.lift ◾ τ
+  := by
+    simp [lift, act, SubstAction.act]; congr; funext; case _ i =>
+    cases i <;> simp [act, SubstAction.act]
+    case _ n =>
+      simp [hcompose_ren, act, SubstAction.act]
+      generalize zdef : σ.inner n = z
+      cases z <;> simp; case _ t =>
+      rw [apply_commute_ren_ren]
+
+  @[simp, grind =]
+  theorem hrewrite_lift_ren
+    [RenMap S S] [RenMap S T] [SubstMap S S] [SubstMap S T]
+    [RenMapId S S] [RenMapCompose S S] [SubstMapRenCommute S T]
+    {k} {σ : Subst S} {τ : Ren T}
+    : (σ ◾ τ).lift k = σ.lift k ◾ τ
+  := by
+    induction k generalizing σ τ
+    case _ => simp
+    case _ i ih =>
+      rw [rewrite_lift_succ]
+      rw [rewrite_lift_succ (k := i)]
+      simp; rw [ih]
 end Subst
 
 @[grind =]
@@ -399,7 +539,7 @@ theorem Subst.lift_compose_ren_right
     rw [<-Ren.lift_of_succ]
 
 theorem Subst.rewrite_lift_compose_k1
-  [RenMap T T] [SubstMap T T] [SubstMapRenComposeLeft T T] [SubstMapRenComposeRight T]
+  [RenMap T T] [SubstMap T T] [SubstMapRenComposeLeft T T] [SubstMapRenComposeRight T T]
   {σ τ : Subst T}
   : (σ ∘ τ).lift = σ.lift ∘ τ.lift
 := by
@@ -408,8 +548,6 @@ theorem Subst.rewrite_lift_compose_k1
   cases x <;> simp [act, SubstAction.act]
   case _ x =>
   cases σ.inner x <;> simp [act, SubstAction.act]; case _ t =>
-  rw [SubstMapRenComposeLeft.apply_ren_compose_left]
-  rw [SubstMapRenComposeRight.apply_ren_compose_right]
   have lem := Subst.compose_commute_succ (τ := τ)
   simp [lift, act, SubstAction.act] at lem
   rw [lem]
@@ -417,7 +555,7 @@ theorem Subst.rewrite_lift_compose_k1
 @[simp, grind =]
 theorem Subst.rewrite_lift_compose
   [RenMap T T] [RenMapId T T] [RenMapCompose T T] [SubstMap T T]
-  [SubstMapRenComposeLeft T T] [SubstMapRenComposeRight T]
+  [SubstMapRenComposeLeft T T] [SubstMapRenComposeRight T T]
   {k} {σ τ : Subst T}
   : (σ ∘ τ).lift k = σ.lift k ∘ τ.lift k
 := by
@@ -438,8 +576,9 @@ macro "subst_solve_stable" : tactic => `(tactic| {
   intro r σ h
   funext; case _ t =>
   induction t generalizing r σ
-  all_goals simp [rmap, smap, *] at *; try simp +instances [*]
-  any_goals solve | (rw [<-h]; simp +instances [Ren.to])
+  all_goals simp [*] at *; try simp +instances [*]
+  all_goals try solve | rw [Subst.apply_stable h]
+  all_goals try solve | (rw [<-h]; simp +instances [Ren.to])
   all_goals try repeat funext; grind
 })
 
